Add generated files

coq/_vc/Pearlite_Example.v
@@ -8,12 +8,18 @@ Open Scope bool_scope.
 Open Scope hacspec_scope.
 Require Import Hacspec_Lib.
 
-Definition ensure_something (x_0 : int8) (y_1 : int8)  `{x_0 = y_1} : bool :=
-  (x_0) =.? (y_1).
+Definition ensure_something
+  (x_2778 : int8)
+  (y_2779 : int8)
+  
+  `{x_2778 = y_2779}
+  : bool :=
+  (x_2778) =.? (y_2779).
 
-Theorem ensures_ensure_something : forall result_2 (x_0 : int8) (y_1 : int8),
- forall {H_0 : x_0 = y_1},
- @ensure_something x_0 y_1 H_0 = result_2 ->
- ~ (result_2 = false).
+Theorem ensures_ensure_something : forall result_2780 (x_2778 : int8) (
+  y_2779 : int8),
+ forall {H_0 : x_2778 = y_2779},
+ @ensure_something x_2778 y_2779 H_0 = result_2780 ->
+ ~ (result_2780 = false).
  Proof. Admitted.
 
