coq/src/Hacspec_Aes128_Gcm.v
@@ -18,17 +18,17 @@ Notation "'aes_gcm_byte_seq_result_t'" := ((
 Definition invalid_tag_v : int8 :=
   @repr WORDSIZE8 1.
 
-Definition pad_aad_msg (aad_278 : byte_seq) (msg_279 : byte_seq) : byte_seq :=
+Definition pad_aad_msg (aad_278 : byte_seq) (msg_279 : byte_seq)  : byte_seq :=
   let laad_280 : uint_size :=
     seq_len (aad_278) in 
   let lmsg_281 : uint_size :=
     seq_len (msg_279) in 
   let pad_aad_282 : uint_size :=
-    (if (((laad_280) %% (usize 16)) =.? (usize 0)):bool then (laad_280) else ((
-          laad_280) + ((usize 16) - ((laad_280) %% (usize 16))))) in 
+    (if (((laad_280) .% (usize 16)) =.? (usize 0)):bool then (laad_280) else ((
+          laad_280) + ((usize 16) - ((laad_280) .% (usize 16))))) in 
   let pad_msg_283 : uint_size :=
-    (if (((lmsg_281) %% (usize 16)) =.? (usize 0)):bool then (lmsg_281) else ((
-          lmsg_281) + ((usize 16) - ((lmsg_281) %% (usize 16))))) in 
+    (if (((lmsg_281) .% (usize 16)) =.? (usize 0)):bool then (lmsg_281) else ((
+          lmsg_281) + ((usize 16) - ((lmsg_281) .% (usize 16))))) in 
   let padded_msg_284 : seq uint8 :=
     seq_new_ (default : uint8) (((pad_aad_282) + (pad_msg_283)) + (
         usize 16)) in 
@@ -53,6 +53,7 @@ Definition encrypt_aes
   (iv_286 : aes_nonce_t)
   (aad_287 : byte_seq)
   (msg_288 : byte_seq)
+  
   : (byte_seq '× gf128_tag_t) :=
   let iv0_289 : aes_nonce_t :=
     array_new_ (default : uint8) (_) in 
@@ -80,6 +81,7 @@ Definition encrypt_aes128
   (iv_297 : aes_nonce_t)
   (aad_298 : byte_seq)
   (msg_299 : byte_seq)
+  
   : (byte_seq '× gf128_tag_t) :=
   encrypt_aes (seq_from_seq (array_to_seq (key_296))) (iv_297) (aad_298) (
     msg_299).
@@ -90,6 +92,7 @@ Definition decrypt_aes
   (aad_302 : byte_seq)
   (cipher_text_303 : byte_seq)
   (tag_304 : gf128_tag_t)
+  
   : aes_gcm_byte_seq_result_t :=
   let iv0_305 : aes_nonce_t :=
     array_new_ (default : uint8) (_) in 
@@ -120,6 +123,7 @@ Definition decrypt_aes128
   (aad_314 : byte_seq)
   (cipher_text_315 : byte_seq)
   (tag_316 : gf128_tag_t)
+  
   : aes_gcm_byte_seq_result_t :=
   decrypt_aes (seq_from_seq (array_to_seq (key_312))) (iv_313) (aad_314) (
     cipher_text_315) (tag_316).
