coq/src/Hacspec_Rsa_Fdh_Vrf.v
@@ -24,47 +24,53 @@ Definition suite_string_v : int_byte_t :=
   one_v.
 
 Definition vrf_mgf1
-  (n_2644 : rsa_int_t)
-  (alpha_2645 : byte_seq)
+  (n_2747 : rsa_int_t)
+  (alpha_2748 : byte_seq)
+  
   : byte_seq_result_t :=
   bind (i2osp (rsa_int_from_literal (@cast _ uint128 _ (byte_size_v))) (
-      @repr WORDSIZE32 4)) (fun mgf_salt1_2646 => bind (i2osp (n_2644) (
-        byte_size_v)) (fun mgf_salt2_2647 => let mgf_salt_2648 : seq uint8 :=
-        seq_concat (mgf_salt1_2646) (mgf_salt2_2647) in 
-      let mgf_string_2649 : seq uint8 :=
+      @repr WORDSIZE32 4)) (fun mgf_salt1_2749 => bind (i2osp (n_2747) (
+        byte_size_v)) (fun mgf_salt2_2750 => let mgf_salt_2751 : seq uint8 :=
+        seq_concat (mgf_salt1_2749) (mgf_salt2_2750) in 
+      let mgf_string_2752 : seq uint8 :=
         seq_concat (seq_concat (array_concat (suite_string_v) (
-              array_to_seq (one_v))) (mgf_salt_2648)) (alpha_2645) in 
-      bind (mgf1 (mgf_string_2649) ((@cast _ uint32 _ (byte_size_v)) - (
-            usize 1))) (fun mgf_2650 => @Ok seq uint8 error_t (mgf_2650)))).
+              array_to_seq (one_v))) (mgf_salt_2751)) (alpha_2748) in 
+      bind (mgf1 (mgf_string_2752) ((@cast _ uint32 _ (byte_size_v)) - (
+            usize 1))) (fun mgf_2753 => @Ok seq uint8 error_t (mgf_2753)))).
 
-Definition prove (sk_2651 : sk_t) (alpha_2652 : byte_seq) : byte_seq_result_t :=
-  let '(n_2653, d_2654) :=
-    (sk_2651) in 
-  bind (vrf_mgf1 (n_2653) (alpha_2652)) (fun em_2655 =>
-    let m_2656 : rsa_int_t :=
-      os2ip (em_2655) in 
-    bind (rsasp1 (sk_2651) (m_2656)) (fun s_2657 => i2osp (s_2657) (
+Definition prove
+  (sk_2754 : sk_t)
+  (alpha_2755 : byte_seq)
+  
+  : byte_seq_result_t :=
+  let '(n_2756, d_2757) :=
+    (sk_2754) in 
+  bind (vrf_mgf1 (n_2756) (alpha_2755)) (fun em_2758 =>
+    let m_2759 : rsa_int_t :=
+      os2ip (em_2758) in 
+    bind (rsasp1 (sk_2754) (m_2759)) (fun s_2760 => i2osp (s_2760) (
         byte_size_v))).
 
-Definition proof_to_hash (pi_string_2658 : byte_seq) : byte_seq_result_t :=
-  let hash_string_2659 : seq uint8 :=
-    array_concat (suite_string_v) (array_concat (two_v) (pi_string_2658)) in 
-  @Ok seq uint8 error_t (array_slice (sha256 (hash_string_2659)) (usize 0) (
+Definition proof_to_hash (pi_string_2761 : byte_seq)  : byte_seq_result_t :=
+  let hash_string_2762 : seq uint8 :=
+    array_concat (suite_string_v) (array_concat (two_v) (pi_string_2761)) in 
+  @Ok seq uint8 error_t (array_slice (sha256 (hash_string_2762)) (usize 0) (
       usize 32)).
 
 Definition verify
-  (pk_2660 : pk_t)
-  (alpha_2661 : byte_seq)
-  (pi_string_2662 : byte_seq)
+  (pk_2763 : pk_t)
+  (alpha_2764 : byte_seq)
+  (pi_string_2765 : byte_seq)
+  
   : byte_seq_result_t :=
-  let '(n_2663, e_2664) :=
-    (pk_2660) in 
-  let s_2665 : rsa_int_t :=
-    os2ip (pi_string_2662) in 
-  bind (rsavp1 (pk_2660) (s_2665)) (fun m_2666 => bind (vrf_mgf1 (n_2663) (
-        alpha_2661)) (fun em_prime_2667 => let m_prime_2668 : rsa_int_t :=
-        os2ip (em_prime_2667) in 
-      (if ((m_2666) =.? (m_prime_2668)):bool then (proof_to_hash (
-            pi_string_2662)) else (@Err seq uint8 error_t (
+  let '(n_2766, e_2767) :=
+    (pk_2763) in 
+  let s_2768 : rsa_int_t :=
+    os2ip (pi_string_2765) in 
+  bind (rsavp1 (pk_2763) (s_2768)) (fun m_2769 => bind (vrf_mgf1 (n_2766) (
+        alpha_2764)) (fun em_prime_2770 => let m_prime_2771 : rsa_int_t :=
+        os2ip (em_prime_2770) in 
+      (if ((m_2769) =.? (m_prime_2771)):bool then (proof_to_hash (
+            pi_string_2765)) else (@Err seq uint8 error_t (
             VerificationFailed))))).
 
